new/golang/defn.v
@@ -1,2 +1,2 @@
 From New.golang.defn Require Export core.
-From New.golang.defn Require Export slice defer chan.
+From New.golang.defn Require Export chan.
